Seperated into files

SeqOfSeq.dfy
@@ -6,97 +6,56 @@ module SeqOfSeq {
 
   /*concatenates a sequence of sequences into a single sequence. 
   Works by adding elements in order from first to last */
-  function method seq_concat<T>(s: seq<seq<T>>): seq<T>
+  function method concat<T>(s: seq<seq<T>>): seq<T>
   decreases |s|
   {
     if |s| == 0 then []
-    else s[0] + seq_concat(s[1..])
-  }
-
-  // turns a sequence of sequences into a single sequence and returns the result
-  function method {:opaque} concat_seq<T>(s: seq<seq<T>>): seq<T>
-  {
-    if |s| == 0 then [] else concat_seq(drop_last(s)) + last(s)
+    else s[0] + concat(s[1..])
   }
 
     /* concatenating two sequences of sequences is equivalent to concatenating
   each sequence of sequences seperately, and then concatenating the two resulting 
   sequences together */
   lemma lemma_concat_adds<T>(a: seq<seq<T>>, b: seq<seq<T>>)
-    ensures seq_concat(a + b) == seq_concat(a) + seq_concat(b)
+    ensures concat(a + b) == concat(a) + concat(b)
   {
     if |a| == 0 {
       assert a + b == b;
     } else {
       calc == {
-        seq_concat(a + b);
+        concat(a + b);
           { assert (a + b)[0] == a[0];  assert (a + b)[1..] == a[1..] + b; }
-        a[0] + seq_concat(a[1..] + b);
-        a[0] + seq_concat(a[1..]) + seq_concat(b);
-        seq_concat(a) + seq_concat(b);
-      }
-    }
-  }
-
-  // proves sequence addition
-  lemma lemma_concat_addition<T>(a: seq<seq<T>>, b: seq<seq<T>>)
-  ensures concat_seq(a + b) == concat_seq(a) + concat_seq(b)
-  {
-    if b == [] {
-      calc {
-        concat_seq(a + b);
-        { assert a + b == a; }
-        concat_seq(a);
-        {
-          reveal_concat_seq();
-          assert concat_seq(b) == [];
-        }
-        concat_seq(a) + concat_seq(b);
-      }
-    } else {
-      calc {
-        concat_seq(a + b);
-        { reveal_concat_seq(); }
-        concat_seq(drop_last(a + b)) + last(a + b);
-        {
-          assert drop_last(a + b) == a + drop_last(b);
-          assert last(a + b) == last(b);
-        }
-        concat_seq(a + drop_last(b)) + last(b);
-        {
-          lemma_concat_addition(a, drop_last(b));
-        }
-        concat_seq(a) + concat_seq(drop_last(b)) + last(b);
-        { reveal_concat_seq(); }
-        concat_seq(a) + concat_seq(b);
+        a[0] + concat(a[1..] + b);
+        a[0] + concat(a[1..]) + concat(b);
+        concat(a) + concat(b);
       }
     }
   }
 
   /* concatenates the sequence of sequences into a single sequence. 
   works by adding elements from last to first */
-  function method seq_concat_reverse<T>(s: seq<seq<T>>): seq<T>
+  function method concat_reverse<T>(s: seq<seq<T>>): seq<T>
   decreases |s|
   {
     if |s| == 0 then []
-    else seq_concat_reverse(drop_last(s)) + last(s)
+    else concat_reverse(drop_last(s)) + last(s)
   }
 
   /* concatenating two reversed sequences of sequences is the same as reversing two 
   sequences of sequences and then adding the two resulting sequences together */
   lemma lemma_concat_reverse_adds<T>(A:seq<seq<T>>, B:seq<seq<T>>)
-  ensures seq_concat_reverse(A + B) == seq_concat_reverse(A) + seq_concat_reverse(B)
+  ensures concat_reverse(A + B) == concat_reverse(A) + concat_reverse(B)
   {
     if |B| == 0 {
-      assert seq_concat_reverse(B) == [];
+      assert concat_reverse(B) == [];
       assert A+B == A;
     } else {
       calc == {
-        seq_concat_reverse(A + B);
+        concat_reverse(A + B);
           { assert last(A + B) == last(B);  assert drop_last(A + B) == A + drop_last(B); }
-        seq_concat_reverse(A + drop_last(B)) + last(B);
-        seq_concat_reverse(A) + seq_concat_reverse(drop_last(B)) + last(B);
-        seq_concat_reverse(A) + seq_concat_reverse(B);
+        concat_reverse(A + drop_last(B)) + last(B);
+        concat_reverse(A) + concat_reverse(drop_last(B)) + last(B);
+        concat_reverse(A) + concat_reverse(B);
       }
     }
   }
@@ -104,19 +63,19 @@ module SeqOfSeq {
   /* both methods of concatenating sequence (starting from front v. starting from back)
   result in the same sequence */
   lemma lemma_concat_and_concat_reverse_are_equivalent<T>(s: seq<seq<T>>)
-    ensures seq_concat(s) == seq_concat_reverse(s)
+    ensures concat(s) == concat_reverse(s)
   {
     if |s| == 0 {
     } else {
       calc == {
-        seq_concat_reverse(s);
-        seq_concat_reverse(drop_last(s)) + last(s);
+        concat_reverse(s);
+        concat_reverse(drop_last(s)) + last(s);
           { lemma_concat_and_concat_reverse_are_equivalent(drop_last(s)); }
-        seq_concat(drop_last(s)) + last(s);
-        seq_concat(drop_last(s)) + seq_concat([last(s)]);
+        concat(drop_last(s)) + last(s);
+        concat(drop_last(s)) + concat([last(s)]);
           { lemma_concat_adds(drop_last(s), [last(s)]); 
         assert s == drop_last(s) + [last(s)]; }
-        seq_concat(s);
+        concat(s);
       }
     }
   }
@@ -125,9 +84,8 @@ module SeqOfSeq {
   each individual inner sequence's length */
   lemma lemma_concat_length_ge_single_element_length<T>(s: seq<seq<T>>, i: int)
   requires 0 <= i < |s|
-  ensures |concat_seq(s)| >= |s[i]|
+  ensures |concat_reverse(s)| >= |s[i]|
   {
-    reveal_concat_seq();
     if i < |s| - 1 {
       lemma_concat_length_ge_single_element_length(s[..|s|-1], i);
     }
@@ -138,9 +96,8 @@ module SeqOfSeq {
   the longest sequence */
   lemma lemma_concat_length_le_mul<T>(s: seq<seq<T>>, j: int)
   requires forall i | 0 <= i < |s| :: |s[i]| <= j
-  ensures |concat_seq(s)| <= |s| * j
+  ensures |concat_reverse(s)| <= |s| * j
   {
-    reveal_concat_seq();
     if |s| == 0 {
     } else {
       lemma_concat_length_le_mul(s[..|s|-1], j);
